llpol.v moved to Type

yalla/llpol.v
@@ -1,15 +1,21 @@
 (* llpol example file for yalla library *)
-(* v 1.0   Olivier Laurent *)
+
+
+(* output in Type *)
+
 
 
 (** * Example of a concrete use of the yalla library: polarized linear logic LLpol *)
 
-Require Import Morphisms.
+Require Import Bool.
+Require Import CMorphisms.
 
 Require Import Injective.
 Require Import List_more.
-Require Import Permutation_more.
-Require Import Permutation_solve.
+Require Import List_Type_more.
+Require Import Permutation_Type.
+Require Import Permutation_Type_more.
+Require Import Permutation_Type_solve.
 
 
 (** ** 0. load the [ll] library *)
@@ -164,7 +170,7 @@ Qed.
 
 Lemma llpol2ll_map_wn_inv : forall l1 l2,
   map formulas.wn l1 = map llpol2ll l2 ->
-    exists l2', l2 = map neg (map wn l2') /\ l1 = map pllpol2ll l2'.
+    { l2' : _ & l2 = map neg (map wn l2') & l1 = map pllpol2ll l2' }.
 Proof with try assumption ; try reflexivity.
 induction l1 ; intros l2 Heq ;
   destruct l2 ; inversion Heq...
@@ -172,7 +178,7 @@ induction l1 ; intros l2 Heq ;
 - apply IHl1 in H1.
   destruct f ; inversion H0 ;
     [ destruct p | destruct n ] ; inversion H0 ; subst.
-  destruct H1 as (l2' & Heq1 & H1) ; subst.
+  destruct H1 as [l2' Heq1 H1] ; subst.
   exists (p :: l2') ; split...
 Qed.
 
@@ -180,10 +186,10 @@ Qed.
 (** ** 3. define proofs *)
 
 (** [ll] restricted to polarized formulas *)
-Inductive llpol : list formula -> Prop :=
+Inductive llpol : list formula -> Type :=
 | ax_r : forall X, llpol (neg (covar X) :: pos (var X) :: nil)
 | ex_r : forall l1 l2, llpol l1 ->
-              Permutation l1 l2 -> llpol l2
+              Permutation_Type l1 l2 -> llpol l2
 | one_r : llpol (pos one :: nil)
 | bot_r : forall l, llpol l -> llpol (neg bot :: l)
 | tens_r : forall P Q l1 l2,
@@ -211,7 +217,7 @@ Inductive llpol : list formula -> Prop :=
               llpol (neg (wn P) :: neg (wn P) :: l) ->
               llpol (neg (wn P) :: l).
 
-Instance llpol_perm : Proper ((@Permutation _) ==> Basics.impl) llpol.
+Instance llpol_perm : Proper ((@Permutation_Type _) ==> Basics.arrow) llpol.
 Proof.
 intros l1 l2 HP pi.
 eapply ex_r ; eassumption.
@@ -221,66 +227,219 @@ Qed.
 (** ** 4. characterize corresponding [ll] fragment *)
 
 (*
-Definition llpol_fragment A := exists B, A = llpol2ll B.
+Lemma llpol2ll_dec : forall A,
+  {B | A = llpol2ll B} + (forall B, A = llpol2ll B -> False).
+Proof with try reflexivity.
+induction A.
+- left ; exists (pos (var a))...
+- left ; exists (neg (covar a))...
+- left ; exists (pos one)...
+- left ; exists (neg bot)...
+- destruct IHA1 as [[[p1 | n1] Heq1] | pi1] ;
+  destruct IHA2 as [[[p2 | n2] Heq2] | pi2] ; subst ;
+    try now
+      (right ; intros B Heq ; 
+       destruct B ; try destruct p ; try destruct n ; inversion Heq ;
+       (try now (destruct n1 ; destruct p1 ; inversion H0)) ;
+       (try now (destruct n2 ; destruct p2 ; inversion H1)) ;
+       (try now (destruct n2 ; destruct p3 ; inversion H1))).
+  + left ; exists (pos (tens p1 p2))...
+  + right ; intros B Heq.
+    destruct B ; try destruct n ; try destruct p ; inversion Heq ; subst.
+    apply (pi2 (pos p3))...
+  + right ; intros B Heq.
+    destruct B ; try destruct n ; try destruct p ; inversion Heq ; subst.
+    apply (pi1 (pos p1))...
+  + right ; intros B Heq.
+    destruct B ; try destruct n ; try destruct p ; inversion Heq ; subst.
+    apply (pi2 (pos p2))...
+- destruct IHA1 as [[[p1 | n1] Heq1] | pi1] ;
+  destruct IHA2 as [[[p2 | n2] Heq2] | pi2] ; subst ;
+    try now
+      (right ; intros B Heq ; 
+       destruct B ; try destruct p ; try destruct n ; inversion Heq ;
+       (try now (destruct n1 ; destruct p1 ; inversion H0)) ;
+       (try now (destruct n2 ; destruct p2 ; inversion H1)) ;
+       (try now (destruct p2 ; destruct n3 ; inversion H1))).
+  + left ; exists (neg (parr n1 n2))...
+  + right ; intros B Heq.
+    destruct B ; try destruct n ; try destruct p ; inversion Heq ; subst.
+    apply (pi2 (neg n3))...
+  + right ; intros B Heq.
+    destruct B ; try destruct n ; try destruct p ; inversion Heq ; subst.
+    apply (pi1 (neg n1))...
+  + right ; intros B Heq.
+    destruct B ; try destruct n ; try destruct p ; inversion Heq ; subst.
+    apply (pi2 (neg n2))...
+- left ; exists (pos zero)...
+- left ; exists (neg top)...
+- destruct IHA1 as [[[p1 | n1] Heq1] | pi1] ;
+  destruct IHA2 as [[[p2 | n2] Heq2] | pi2] ; subst ;
+    try now
+      (right ; intros B Heq ; 
+       destruct B ; try destruct p ; try destruct n ; inversion Heq ;
+       (try now (destruct n1 ; destruct p1 ; inversion H0)) ;
+       (try now (destruct n2 ; destruct p2 ; inversion H1)) ;
+       (try now (destruct n2 ; destruct p3 ; inversion H1))).
+  + left ; exists (pos (aplus p1 p2))...
+  + right ; intros B Heq.
+    destruct B ; try destruct n ; try destruct p ; inversion Heq ; subst.
+    apply (pi2 (pos p3))...
+  + right ; intros B Heq.
+    destruct B ; try destruct n ; try destruct p ; inversion Heq ; subst.
+    apply (pi1 (pos p1))...
+  + right ; intros B Heq.
+    destruct B ; try destruct n ; try destruct p ; inversion Heq ; subst.
+    apply (pi2 (pos p2))...
+- destruct IHA1 as [[[p1 | n1] Heq1] | pi1] ;
+  destruct IHA2 as [[[p2 | n2] Heq2] | pi2] ; subst ;
+    try now
+      (right ; intros B Heq ; 
+       destruct B ; try destruct p ; try destruct n ; inversion Heq ;
+       (try now (destruct n1 ; destruct p1 ; inversion H0)) ;
+       (try now (destruct n2 ; destruct p2 ; inversion H1)) ;
+       (try now (destruct p2 ; destruct n3 ; inversion H1))).
+  + left ; exists (neg (awith n1 n2))...
+  + right ; intros B Heq.
+    destruct B ; try destruct n ; try destruct p ; inversion Heq ; subst.
+    apply (pi2 (neg n3))...
+  + right ; intros B Heq.
+    destruct B ; try destruct n ; try destruct p ; inversion Heq ; subst.
+    apply (pi1 (neg n1))...
+  + right ; intros B Heq.
+    destruct B ; try destruct n ; try destruct p ; inversion Heq ; subst.
+    apply (pi2 (neg n2))...
+- destruct IHA as [[[p | n] Heq] | pi] ; subst.
+  + right ; intros B Heq.
+    destruct B ; try destruct p0 ; try destruct n ;
+      destruct p ; inversion Heq.
+  + left ; exists (pos (oc n))...
+  + right ; intros B Heq.
+    destruct B ; try destruct p ; inversion Heq ; subst...
+    * apply (pi (neg n))...
+    * destruct n ; inversion H0.
+- destruct IHA as [[[p | n] Heq] | pi] ; subst.
+  + left ; exists (neg (wn p))...
+  + right ; intros B Heq.
+    destruct B ; try destruct n0 ; try destruct p ;
+      destruct n ; inversion Heq.
+  + right ; intros B Heq.
+    destruct B ; try destruct n ; inversion Heq ; subst...
+    * destruct p ; inversion H0.
+    * apply (pi (pos p))...
+Qed.
+
+Definition llpol_fragment A :=
+match (llpol2ll_dec A) with
+| inl _ => true
+| inr _ => false
+end.
 
 Lemma llpol_is_fragment : ll.fragment llpol_fragment.
-Proof.
+Proof with try reflexivity.
 intros A HfA B Hsf.
 induction Hsf ;
-  try (apply IHHsf ;
-       destruct HfA ;
-       destruct x ; inversion H ;
-       [ destruct p ; inversion H
-       | destruct n ; inversion H ] ;
-       try (eexists (pos _) ; reflexivity) ;
-       try (eexists (neg _) ; reflexivity)).
-assumption.
+unfold llpol_fragment in HfA ;
+(destruct (llpol2ll_dec A) ;
+  [ destruct s as [A' Heq] ; subst ;
+    unfold llpol_fragment ;
+    destruct (llpol2ll_dec (llpol2ll A')) ;
+    [ | exfalso ; eapply f ]
+  | ])...
+- inversion HfA.
+- destruct (llpol2ll_dec (formulas.tens B C)) ; try now inversion HfA.
+  destruct s as [B' Heq].
+  destruct B' ; [ destruct p | destruct n ] ; inversion Heq ; subst.
+  apply IHHsf.
+  unfold llpol_fragment ; destruct (llpol2ll_dec (pllpol2ll p1)) ;
+    [ | exfalso ; apply (f0 (pos p1)) ]...
+- destruct (llpol2ll_dec (formulas.tens C B)) ; try now inversion HfA.
+  destruct s as [B' Heq].
+  destruct B' ; [ destruct p | destruct n ] ; inversion Heq ; subst.
+  apply IHHsf.
+  unfold llpol_fragment ; destruct (llpol2ll_dec (pllpol2ll p2)) ;
+    [ | exfalso ; apply (f0 (pos p2)) ]...
+- destruct (llpol2ll_dec (formulas.parr B C)) ; try now inversion HfA.
+  destruct s as [B' Heq].
+  destruct B' ; [ destruct p | destruct n ] ; inversion Heq ; subst.
+  apply IHHsf.
+  unfold llpol_fragment ; destruct (llpol2ll_dec (nllpol2ll n1)) ;
+    [ | exfalso ; apply (f0 (neg n1)) ]...
+- destruct (llpol2ll_dec (formulas.parr C B)) ; try now inversion HfA.
+  destruct s as [B' Heq].
+  destruct B' ; [ destruct p | destruct n ] ; inversion Heq ; subst.
+  apply IHHsf.
+  unfold llpol_fragment ; destruct (llpol2ll_dec (nllpol2ll n2)) ;
+    [ | exfalso ; apply (f0 (neg n2)) ]...
+- destruct (llpol2ll_dec (formulas.aplus B C)) ; try now inversion HfA.
+  destruct s as [B' Heq].
+  destruct B' ; [ destruct p | destruct n ] ; inversion Heq ; subst.
+  apply IHHsf.
+  unfold llpol_fragment ; destruct (llpol2ll_dec (pllpol2ll p1)) ;
+    [ | exfalso ; apply (f0 (pos p1)) ]...
+- destruct (llpol2ll_dec (formulas.aplus C B)) ; try now inversion HfA.
+  destruct s as [B' Heq].
+  destruct B' ; [ destruct p | destruct n ] ; inversion Heq ; subst.
+  apply IHHsf.
+  unfold llpol_fragment ; destruct (llpol2ll_dec (pllpol2ll p2)) ;
+    [ | exfalso ; apply (f0 (pos p2)) ]...
+- destruct (llpol2ll_dec (formulas.awith B C)) ; try now inversion HfA.
+  destruct s as [B' Heq].
+  destruct B' ; [ destruct p | destruct n ] ; inversion Heq ; subst.
+  apply IHHsf.
+  unfold llpol_fragment ; destruct (llpol2ll_dec (nllpol2ll n1)) ;
+    [ | exfalso ; apply (f0 (neg n1)) ]...
+- destruct (llpol2ll_dec (formulas.awith C B)) ; try now inversion HfA.
+  destruct s as [B' Heq].
+  destruct B' ; [ destruct p | destruct n ] ; inversion Heq ; subst.
+  apply IHHsf.
+  unfold llpol_fragment ; destruct (llpol2ll_dec (nllpol2ll n2)) ;
+    [ | exfalso ; apply (f0 (neg n2)) ]...
+- destruct (llpol2ll_dec (formulas.oc B)) ; try now inversion HfA.
+  destruct s as [B' Heq].
+  destruct B' ; [ destruct p | destruct n ] ; inversion Heq ; subst.
+  apply IHHsf.
+  unfold llpol_fragment ; destruct (llpol2ll_dec (nllpol2ll n)) ;
+    [ | exfalso ; apply (f0 (neg n)) ]...
+- destruct (llpol2ll_dec (formulas.wn B)) ; try now inversion HfA.
+  destruct s as [B' Heq].
+  destruct B' ; [ destruct p | destruct n ] ; inversion Heq ; subst.
+  apply IHHsf.
+  unfold llpol_fragment ; destruct (llpol2ll_dec (pllpol2ll p)) ;
+    [ | exfalso ; apply (f0 (pos p)) ]...
 Qed.
 *)
 
 (** cut / axioms / mix0 / mix2 / permutation *)
-Definition pfrag_mell := ll.mk_pfrag false (fun _ => False) false false true.
-(*                                   cut   axioms           mix0  mix2  perm  *)
+Definition pfrag_mell := ll.mk_pfrag false ll.NoAxioms false false true.
+(*                                   cut   axioms      mix0  mix2  perm  *)
 
 
 (** ** 5. prove equivalence of proof predicates *)
 
 Lemma llpol2llpolfrag : forall l, llpol l ->
-  exists s, ll.ll pfrag_mell (map llpol2ll l) s.
+  ll.ll pfrag_mell (map llpol2ll l).
 Proof with try eassumption ; try reflexivity.
-intros l pi.
-induction pi ;
-  try destruct IHpi as [s' pi'] ;
-  try destruct IHpi1 as [s1' pi1'] ;
-  try destruct IHpi2 as [s2' pi2'] ;
-  eexists ; simpl ; rewrite ? map_app.
-- apply ll.ax_r.
+intros l pi ; induction pi ; try now (constructor ; intuition).
 - eapply ll.ex_r...
-  apply Permutation_map...
-- eapply ll.one_r.
-- eapply ll.bot_r...
+  apply Permutation_Type_map...
 - eapply ll.ex_r.
-  + apply (ll.tens_r _ _ _ _ _ _ _ pi1' pi2').
-  + simpl ; perm_solve.
-- apply ll.parr_r...
-- apply ll.top_r.
-- apply ll.plus_r1...
-- apply ll.plus_r2...
-- apply ll.with_r...
-- rewrite llpol2ll_map_wn.
+  + apply (ll.tens_r _ _ _ _ _ IHpi1 IHpi2).
+  + simpl ; perm_Type_solve.
+- simpl ; rewrite ? map_app.
+  rewrite llpol2ll_map_wn.
   apply ll.oc_r.
   rewrite <- llpol2ll_map_wn...
-- apply ll.de_r...
-- apply ll.wk_r...
-- rewrite <- (app_nil_l (map _ _)).
+- simpl ; rewrite ? map_app.
+  rewrite <- (app_nil_l (map _ _)).
   change nil with (map formulas.wn nil).
   apply ll.co_r...
 Qed.
 
-Lemma llpolfrag2llpol : forall l s,
-  ll.ll pfrag_mell (map llpol2ll l) s -> llpol l.
+Lemma llpolfrag2llpol : forall l,
+  ll.ll pfrag_mell (map llpol2ll l) -> llpol l.
 Proof with try reflexivity.
-intros l s pi.
+intros l pi.
 remember (map llpol2ll l) as l0.
 revert l Heql0 ; induction pi ; intros l' Heql0 ; subst ;
   try (now (destruct l' ; inversion Heql0 ;
@@ -289,7 +448,7 @@ revert l Heql0 ; induction pi ; intros l' Heql0 ; subst ;
             constructor ;
             apply IHpi ; reflexivity)) ;
   try (now inversion f).
-- decomp_map Heql0 ; subst.
+- decomp_map_Type Heql0 ; subst.
   destruct l1 ; inversion Heql4.
   destruct x ; inversion Heql2 ;
     [ destruct p | destruct n ] ; inversion Heql2.
@@ -297,9 +456,9 @@ revert l Heql0 ; induction pi ; intros l' Heql0 ; subst ;
     [destruct p | destruct n ] ; inversion Heql0.
   subst ; subst.
   apply ax_r.
-- simpl in H.
-  apply Permutation_map_inv in H.
-  destruct H as (l'' & Heq & HP) ; subst.
+- simpl in p.
+  apply Permutation_Type_map_inv in p.
+  destruct p as [l'' Heq HP] ; subst.
   symmetry in HP.
   eapply ex_r ; [ | eassumption ].
   apply IHpi...
@@ -308,14 +467,14 @@ revert l Heql0 ; induction pi ; intros l' Heql0 ; subst ;
     [ destruct p | destruct n ] ; inversion H0.
   destruct l' ; inversion H1.
   apply one_r.
-- decomp_map Heql0 ; subst.
+- decomp_map_Type Heql0 ; subst.
   destruct x ; inversion Heql2 ;
     [ destruct p | destruct n ] ; inversion Heql2 ; subst.
   eapply ex_r.
   apply tens_r.
   + apply IHpi1...
   + apply IHpi2...
-  + perm_solve.
+  + perm_Type_solve.
 - destruct l' ; inversion Heql0.
   destruct f ; inversion H0 ;
     [ destruct p | destruct n ] ; inversion H0 ; subst.
@@ -326,19 +485,20 @@ revert l Heql0 ; induction pi ; intros l' Heql0 ; subst ;
   destruct f ; inversion H0 ; 
     [destruct p | destruct n ] ; inversion H0 ; subst.
   apply llpol2ll_map_wn_inv in H1.
-  destruct H1 as (l'' & Heq1 & Heq2) ; subst.
+  destruct H1 as [l'' Heq1 Heq2] ; subst.
   apply oc_r.
   apply IHpi.
   simpl ; rewrite llpol2ll_map_wn...
 - destruct l' ; inversion Heql0.
   destruct f ; inversion H0 ;
     [ destruct p | destruct n ] ; inversion H0 ; subst.
-  decomp_map H1 ; subst.
+  decomp_map_Type H1 ; subst.
   apply co_r.
   apply llpol2ll_map_wn_inv in H4.
-  destruct H4 as (l'' & Heq1 & Heq2) ; subst.
+  destruct H4 as [l'' Heq1 Heq2] ; simpl in Heq1 ; subst.
   eapply ex_r.
   + apply IHpi...
+    simpl.
     rewrite <- llpol2ll_map_wn.
     replace (formulas.wn (pllpol2ll p)
                             :: map llpol2ll (map neg (map wn l''))
@@ -346,8 +506,8 @@ revert l Heql0 ; induction pi ; intros l' Heql0 ; subst ;
       with (map llpol2ll (neg (wn p) :: map neg (map wn l'')
                         ++ neg (wn p) :: l2))...
     list_simpl...
-  + perm_solve.
-- inversion H.
+  + perm_Type_solve.
+- inversion a.
 Qed.
 
 
@@ -358,12 +518,10 @@ Qed.
 Lemma ax_gen_r : forall A, llpol (dual A :: A :: nil).
 Proof.
 intro A.
-destruct (@ll.ax_exp pfrag_mell (formulas.dual (llpol2ll A)))
-  as [s Hax].
-rewrite formulas.bidual in Hax.
-rewrite llpol2ll_dual in Hax.
-eapply llpolfrag2llpol.
-eassumption.
+eapply ex_r ; [ | apply Permutation_Type_swap ].
+apply llpolfrag2llpol.
+simpl ; rewrite <- llpol2ll_dual.
+apply ll.ax_exp.
 Qed.
 
 (** *** cut elimination *)
@@ -372,14 +530,13 @@ Lemma cut_r : forall A l1 l2,
   llpol (A :: l1) -> llpol (dual A :: l2) -> llpol (l1 ++ l2).
 Proof with try eassumption.
 intros A l1 l2 pi1 pi2.
-destruct (llpol2llpolfrag _ pi1) as [s1 pi1'] ; simpl in pi1'.
-destruct (llpol2llpolfrag _ pi2) as [s2 pi2'] ; simpl in pi2'.
-eapply ll.cut_r_axfree in pi1' ;
+apply llpol2llpolfrag in pi1 ; simpl in pi1.
+apply llpol2llpolfrag in pi2 ; simpl in pi2.
+eapply ll.cut_r_axfree in pi1 ;
   [ | | rewrite llpol2ll_dual ]...
-- destruct pi1' as [s pi].
-  rewrite <- map_app in pi.
+- rewrite <- map_app in pi1.
   eapply llpolfrag2llpol...
-- intros l Hax ; inversion Hax.
+- intros Hax ; inversion Hax.
 Qed.
 
 
@@ -390,7 +547,7 @@ Lemma par_inv : forall N M l,
 Proof with try assumption.
 intros N M l pi.
 rewrite <- (app_nil_l l).
-eapply ex_r ; [ | apply perm_swap ].
+eapply ex_r ; [ | apply Permutation_Type_swap ].
 rewrite 2 app_comm_cons.
 eapply cut_r.
 - rewrite <- (app_nil_l (neg N :: nil)).
@@ -432,165 +589,217 @@ Qed.
 
 (** Polarized sequents are those with at most one positive formula. *)
 Definition polsequent l :=
-     (exists l0, l = map neg l0)
-  \/ (exists l0 P, Permutation l (pos P :: (map neg l0))).
+ sum { l0 | l = map neg l0 }
+     { lP & Permutation_Type l (pos (snd lP) :: (map neg (fst lP))) }.
 
-(*
 Lemma uniq_polsequent : forall l1 l2 P1 P2,
-  Permutation (pos P1 :: map neg l1) (pos P2 :: map neg l2) ->
-    P1 = P2 /\ Permutation l1 l2.
+  Permutation_Type (pos P1 :: l1) (pos P2 :: map neg l2) ->
+    { l1' : _ & l1 = map neg l1' & prod (P1 = P2) (Permutation_Type l1' l2) }.
 Proof with try eassumption ; try reflexivity.
 intros l1 l2 P1 P2 HP.
 assert (HP' := HP).
-apply Permutation_vs_cons_inv in HP'.
-destruct HP' as (l' & l'' & Heq).
-destruct l' ; inversion Heq.
-- split...
-  rewrite H0 in HP.
-  apply Permutation_cons_inv in HP.
-  apply Permutation_map_inv_inj in HP...
-  intros N M Hneg.
-  inversion Hneg...
-- symmetry in H1.
-  exfalso.
+symmetry in HP'.
+apply Permutation_Type_vs_cons_inv in HP'.
+destruct HP' as ((l' & l'') & Heq) ; simpl in Heq.
+destruct l' ; inversion Heq ; subst.
+- apply Permutation_Type_cons_inv in HP.
+  apply Permutation_Type_map_inv in HP.
+  destruct HP as [l Heq' HP'] ; subst.
+  exists l ; [ | split ]...
+  symmetry...
+- exfalso.
+  symmetry in H1.
   decomp_map H1.
   inversion H1.
 Qed.
 
+(*
 Lemma polsequent_app : forall l1 l2,
   polsequent (l1 ++ l2) ->
-    exists l, (l2 = map neg l /\ polsequent l1)
-           \/ (l1 = map neg l /\ polsequent l2).
+    { l & sum (prod (l2 = map neg l) (polsequent l1))
+              (prod (l1 = map neg l) (polsequent l2)) }.
 Proof with try eassumption ; try reflexivity.
 intros l1 l2 Hi.
 assert (Hi' := Hi).
-destruct Hi' as [ (l0 & Hi') | (l0 & P & Hi') ].
-- decomp_map Hi' ; subst.
+destruct Hi' as [ (l0 & Hi') | ((l0 & P) & Hi') ].
+- decomp_map_Type Hi' ; subst.
   exists l4 ; left ; split...
   left ; eexists...
 - assert (Hi'' := Hi').
-  apply Permutation_vs_cons_inv in Hi'.
-  destruct Hi' as (l3 & l4 & Heq).
-  dichot_elt_app_exec Heq ; subst.
+  apply Permutation_Type_vs_cons_inv in Hi'.
+  destruct Hi' as ((l3 & l4) & Heq).
+  dichot_Type_elt_app_exec Heq ; subst.
   + list_simpl in Hi''.
     symmetry in Hi''.
-    apply Permutation_cons_app_inv in Hi''.
+    apply Permutation_Type_cons_app_inv in Hi''.
     symmetry in Hi''.
-    apply Permutation_map_inv in Hi''.
-    destruct Hi'' as (l' & Heq & HP).
-    decomp_map Heq ; subst.
+    apply Permutation_Type_map_inv in Hi''.
+    destruct Hi'' as [l' Heq HP].
+    decomp_map_Type Heq ; subst.
     eexists ; left ; split...
-    right ; exists (l4 ++ l6) ; exists P ; perm_solve.
+    right ; exists (l5 ++ l7, P) ; perm_Type_solve.
   + symmetry in Hi''.
     rewrite app_assoc in Hi''.
-    apply Permutation_cons_app_inv in Hi''.
+    apply Permutation_Type_cons_app_inv in Hi''.
     list_simpl in Hi''.
     symmetry in Hi''.
-    apply Permutation_map_inv in Hi''.
-    destruct Hi'' as (l' & Heq & HP).
-    decomp_map Heq ; subst.
+    apply Permutation_Type_map_inv in Hi''.
+    destruct Hi'' as [l' Heq HP].
+    decomp_map_Type Heq ; subst.
     eexists ; right ; split...
-    right ; exists (l6 ++ l7) ; exists P ; perm_solve.
+    right ; exists (l7 ++ l8, P) ; perm_Type_solve.
 Qed.
 *)
 
 Lemma polsequent_neg_add : forall N l,
   polsequent l -> polsequent (neg N :: l).
 Proof.
-intros N l [ (l0 & Heq) | (l0 & P & HP) ] ; subst.
+intros N l [ (l0 & Heq) | ((l0 & P) & HP) ] ; subst.
 - left ; exists (N :: l0) ; reflexivity.
 - assert (HP' := HP).
-  apply Permutation_vs_cons_inv in HP'.
-  destruct HP' as (l2 & l3 & Heq) ; subst.
+  apply Permutation_Type_vs_cons_inv in HP'.
+  destruct HP' as ((l2 & l3) & Heq) ; subst.
   symmetry in HP.
-  apply Permutation_cons_app_inv in HP.
+  apply Permutation_Type_cons_app_inv in HP.
   symmetry in HP.
-  apply Permutation_map_inv in HP.
-  destruct HP as (l1 & Heq' & _).
-  list_simpl in Heq' ; decomp_map Heq' ; subst.
-  right ; exists (N :: l4 ++ l5) ; exists P ; perm_solve.
+  apply Permutation_Type_map_inv in HP.
+  destruct HP as [l1 Heq' _].
+  list_simpl in Heq' ; decomp_map_Type Heq' ; subst.
+  right ; exists (N :: l4 ++ l5, P) ; perm_Type_solve.
 Qed.
 
 Lemma polsequent_neg_rem : forall N l,
   polsequent (neg N :: l) -> polsequent l.
 Proof.
 intros N l Hpol.
-destruct Hpol as [ (l0 & Heq) | (l0 & P & HP) ] ; subst.
+destruct Hpol as [ (l0 & Heq) | ((l0 & P) & HP) ] ; subst.
 - destruct l0 ; inversion Heq.
   left ; exists l0 ; reflexivity.
 - assert (HP' := HP).
-  apply Permutation_vs_cons_inv in HP'.
-  destruct HP' as (l2 & l3 & Heq).
+  apply Permutation_Type_vs_cons_inv in HP'.
+  destruct HP' as ((l2 & l3) & Heq).
   destruct l2 ; inversion Heq ; subst.
   symmetry in HP.
   rewrite app_comm_cons in HP.
-  apply Permutation_cons_app_inv in HP.
+  apply Permutation_Type_cons_app_inv in HP.
   symmetry in HP.
-  apply Permutation_map_inv in HP.
-  destruct HP as (l1 & Heq' & _).
-  list_simpl in Heq' ; decomp_map Heq' ; subst.
-  right ; exists (l5 ++ l6) ; exists P ; perm_solve.
+  apply Permutation_Type_map_inv in HP.
+  destruct HP as [l1 Heq' _].
+  list_simpl in Heq' ; decomp_map_Type Heq' ; subst.
+  right ; exists (l5 ++ l6, P) ; perm_Type_solve.
 Qed.
 
 Lemma polsequent_pos_rem : forall P l,
-  polsequent (pos P :: l) -> exists l', l = map neg l'.
+  polsequent (pos P :: l) -> { l' | l = map neg l' }.
 Proof with try reflexivity.
 intros P l Hs.
-destruct Hs as [ (l0 & Heq) | (l0 & Q & HP) ].
-- decomp_map Heq ; inversion Heq1.
+destruct Hs as [ (l0 & Heq) | ((l0 & Q) & HP) ].
+- decomp_map_Type Heq ; inversion Heq1.
 - assert (HP' := HP).
-  apply Permutation_vs_cons_inv in HP'.
-  destruct HP' as (l' & l'' & Heq).
+  apply Permutation_Type_vs_cons_inv in HP'.
+  destruct HP' as ((l' & l'') & Heq).
   destruct l' ; inversion Heq ; subst.
-  + apply Permutation_cons_inv in HP.
-    apply Permutation_map_inv in HP...
-    destruct HP as (l' & Heq' & HP') ; subst.
+  + apply Permutation_Type_cons_inv in HP.
+    apply Permutation_Type_map_inv in HP...
+    destruct HP as [l' Heq' HP'] ; subst.
     eexists...
   + exfalso.
     symmetry in HP.
     rewrite app_comm_cons in HP.
-    apply Permutation_cons_app_inv in HP.
+    apply Permutation_Type_cons_app_inv in HP.
     symmetry in HP.
-    apply Permutation_map_inv in HP.
-    destruct HP as (l2 & Heq' & HP').
+    apply Permutation_Type_map_inv in HP.
+    destruct HP as [l2 Heq' HP'].
     destruct l2 ; inversion Heq'.
 Qed.
 
+Lemma polsequent_dec : forall l, polsequent l + (polsequent l -> False).
+Proof.
+induction l.
+- left ; left ; exists nil ; reflexivity.
+- destruct a.
+  + destruct IHl.
+    * destruct p0.
+      -- destruct s as [l0 Heq] ; subst.
+         left ; right ; exists (l0,p) ; reflexivity.
+      -- destruct s as [[l0 P] HP].
+         right ; intros Hps ; destruct Hps.
+         ++ destruct s as [l1 Heq] ; subst.
+            destruct l1 ; inversion Heq.
+         ++ destruct s as [[l1 Q] HP'].
+            apply uniq_polsequent in HP'.
+            destruct HP' as [l' Heq [Heq' HP']] ; subst.
+            simpl in HP ; symmetry in HP.
+            apply Permutation_Type_map_inv in HP.
+            destruct HP as [l Heq _].
+            destruct l ; inversion Heq.
+    * right ; intros Hps.
+      apply f.
+      left ; eapply polsequent_pos_rem ; eassumption.
+  + destruct IHl.
+    * left.
+      apply polsequent_neg_add ; assumption.
+    * right ; intros Hps.
+      apply f ; clear f.
+      eapply polsequent_neg_rem ; eassumption.
+Qed.
+
+Definition polsequent_bool l :=
+match polsequent_dec l with
+| inl _ => true
+| inr _ => false
+end.
+
+Lemma true_polsequent : forall l,
+  polsequent_bool l = true -> polsequent l.
+Proof.
+intros l Hb ; unfold polsequent_bool in Hb ; destruct (polsequent_dec l).
+- assumption.
+- inversion Hb.
+Qed.
+
+Lemma polsequent_true : forall l,
+  polsequent l -> polsequent_bool l = true.
+Proof.
+intros l Hp.
+unfold polsequent_bool ; destruct (polsequent_dec l) ; intuition.
+Qed.
+
 (** Version of [llpol] with a predicate parameter for constraining sequents inside proofs. *)
-Inductive llpol_ps (PS : list formula -> Prop) : list formula -> Prop :=
-| ax_ps_r : forall X, PS (neg (covar X) :: pos (var X) :: nil) ->
+Inductive llpol_ps PS : list formula -> Type :=
+| ax_ps_r : forall X, is_true (PS (neg (covar X) :: pos (var X) :: nil)) ->
                 llpol_ps PS (neg (covar X) :: pos (var X) :: nil)
-| ex_ps_r : forall l1 l2, PS l2 ->
-                llpol_ps PS l1 -> Permutation l1 l2 -> llpol_ps PS l2
-| one_ps_r : PS (pos one :: nil) -> llpol_ps PS (pos one :: nil)
-| bot_ps_r : forall l, PS (neg bot :: l) ->
+| ex_ps_r : forall l1 l2, is_true (PS l2) ->
+                llpol_ps PS l1 -> Permutation_Type l1 l2 -> llpol_ps PS l2
+| one_ps_r : is_true (PS (pos one :: nil)) -> llpol_ps PS (pos one :: nil)
+| bot_ps_r : forall l, is_true (PS (neg bot :: l)) ->
                 llpol_ps PS l -> llpol_ps PS (neg bot :: l)
-| tens_ps_r : forall P Q l1 l2, PS (pos (tens P Q) :: l1 ++ l2) ->
+| tens_ps_r : forall P Q l1 l2, is_true (PS (pos (tens P Q) :: l1 ++ l2)) ->
                 llpol_ps PS (pos P :: l1) -> llpol_ps PS (pos Q :: l2) ->
                 llpol_ps PS (pos (tens P Q) :: l1 ++ l2)
-| parr_ps_r : forall N M l, PS (neg (parr N M) :: l) -> 
+| parr_ps_r : forall N M l, is_true (PS (neg (parr N M) :: l)) ->
                 llpol_ps PS (neg N :: neg M :: l) ->
                 llpol_ps PS (neg (parr N M) :: l)
-| top_ps_r : forall l, PS (neg top :: l) -> llpol_ps PS (neg top :: l)
-| plus_ps_r1 : forall P Q l, PS (pos (aplus P Q) :: l) ->
+| top_ps_r : forall l, is_true (PS (neg top :: l)) -> llpol_ps PS (neg top :: l)
+| plus_ps_r1 : forall P Q l, is_true (PS (pos (aplus P Q) :: l)) ->
                 llpol_ps PS (pos P :: l)-> llpol_ps PS (pos (aplus P Q) :: l)
-| plus_ps_r2 : forall P Q l, PS (pos (aplus Q P) :: l) ->
+| plus_ps_r2 : forall P Q l, is_true (PS (pos (aplus Q P) :: l)) ->
                 llpol_ps PS (pos P :: l)-> llpol_ps PS (pos (aplus Q P) :: l)
-| with_ps_r : forall N M l, PS (neg (awith N M) :: l) ->
+| with_ps_r : forall N M l, is_true (PS (neg (awith N M) :: l)) ->
                 llpol_ps PS (neg N :: l) -> llpol_ps PS (neg M :: l) ->
                 llpol_ps PS (neg (awith N M) :: l)
-| oc_ps_r : forall N l, PS (pos (oc N) :: map neg (map wn l)) ->
+| oc_ps_r : forall N l, is_true (PS (pos (oc N) :: map neg (map wn l))) ->
                 llpol_ps PS (neg N :: map neg (map wn l)) ->
                 llpol_ps PS (pos (oc N) :: map neg (map wn l))
-| de_ps_r : forall P l, PS (neg (wn P) :: l) ->
+| de_ps_r : forall P l, is_true (PS (neg (wn P) :: l)) ->
                 llpol_ps PS (pos P :: l) -> llpol_ps PS (neg (wn P) :: l)
-| wk_ps_r : forall P l, PS (neg (wn P) :: l) ->
+| wk_ps_r : forall P l, is_true (PS (neg (wn P) :: l)) ->
                 llpol_ps PS l -> llpol_ps PS (neg (wn P) :: l)
-| co_ps_r : forall P l, PS (neg (wn P) :: l) ->
+| co_ps_r : forall P l, is_true (PS (neg (wn P) :: l)) ->
                 llpol_ps PS (neg (wn P) :: neg (wn P) :: l) ->
                 llpol_ps PS (neg (wn P) :: l).
 
-Lemma llpol_ps_is_ps : forall l PS, llpol_ps PS l -> PS l.
+Lemma llpol_ps_is_ps : forall l PS, llpol_ps PS l -> is_true (PS l).
 Proof.
 intros l PS Hll.
 inversion Hll ; assumption.
@@ -607,7 +816,7 @@ induction pi ;
 eapply ex_r...
 Qed.
 
-Lemma llpol_is_llpol_ps : forall l, llpol l -> llpol_ps (fun _ => True) l.
+Lemma llpol_is_llpol_ps : forall l, llpol l -> llpol_ps (fun _ => true) l.
 Proof with try eassumption ; try reflexivity.
 intros l pi.
 induction pi ;
@@ -616,551 +825,528 @@ eapply ex_ps_r...
 Qed.
 
 (** Formulas with [top] below negative connectives only. Such formulas are equivalent to [top]. *)
-Inductive top_surf : nformula -> Prop :=
+Inductive top_surf : nformula -> Type :=
 | top_s : top_surf top
 | par_ls : forall N M, top_surf N -> top_surf (parr N M)
 | par_rs : forall N M, top_surf N -> top_surf (parr M N)
 | with_s : forall N M, top_surf N -> top_surf M -> top_surf (awith N M).
 
 Lemma top_imp_top_surf_ps : forall N l,
-  top_surf N -> polsequent l -> llpol_ps polsequent (neg N :: l).
+  top_surf N -> polsequent l -> llpol_ps polsequent_bool (neg N :: l).
 Proof with try eassumption.
 induction N ; intros l Ht Hp ; inversion Ht ; subst.
 - eapply IHN1 in H0.
   + apply parr_ps_r...
     apply llpol_ps_is_ps in H0.
+    apply true_polsequent in H0.
+    apply polsequent_true.
     apply polsequent_neg_add.
     eapply polsequent_neg_rem.
     eapply polsequent_neg_rem...
   + apply polsequent_neg_add...
 - eapply IHN2 in H0.
-  apply parr_ps_r ; [ | eapply ex_ps_r ; [ | | now apply perm_swap ]]...
+  apply parr_ps_r ; [ | eapply ex_ps_r ; [ | | now apply Permutation_Type_swap ]]...
   + apply llpol_ps_is_ps in H0.
+    apply true_polsequent in H0.
+    apply polsequent_true.
     apply polsequent_neg_add.
     eapply polsequent_neg_rem.
     eapply polsequent_neg_rem...
   + apply llpol_ps_is_ps in H0.
+    apply true_polsequent in H0.
+    apply polsequent_true.
     apply polsequent_neg_add.
     apply polsequent_neg_add.
     eapply polsequent_neg_rem.
     eapply polsequent_neg_rem...
   + apply polsequent_neg_add...
 - apply top_ps_r.
+    apply polsequent_true.
   apply polsequent_neg_add...
 - apply with_ps_r.
-  + apply polsequent_neg_add...
+  + apply polsequent_true.
+    apply polsequent_neg_add...
   + eapply IHN1 in H1...
   + eapply IHN2 in H2...
 Qed.
 
 Lemma bipos_top_surf : forall l,
-  llpol l -> forall P Q l', Permutation l (pos P :: pos Q :: l') ->
-    exists N l1 l2, l' = l1 ++ neg N :: l2 /\ top_surf N.
+  llpol l -> forall P Q l', Permutation_Type l (pos P :: pos Q :: l') ->
+    { Nll : _ & l' = fst (snd Nll) ++ neg (fst Nll) :: snd (snd Nll)
+              & top_surf (fst Nll) }.
 Proof with try assumption ; try reflexivity.
 intros l pi ; induction pi ; intros P' Q' l' HP.
-- apply Permutation_length_2_inv in HP.
+- apply Permutation_Type_length_2_inv in HP.
   destruct HP as [ HP | HP ] ; inversion HP.
 - eapply IHpi.
-  etransitivity ; [ apply H | apply HP ].
-- apply Permutation_length_1_inv in HP.
+  etransitivity ; [ apply p | apply HP ].
+- apply Permutation_Type_length_1_inv in HP.
   inversion HP.
 - assert (HP' := HP).
   symmetry in HP'.
-  apply Permutation_vs_cons_inv in HP'.
-  destruct HP' as (l2 & l3 & Heq).
+  apply Permutation_Type_vs_cons_inv in HP'.
+  destruct HP' as ((l2 & l3) & Heq).
   destruct l2 ; inversion Heq.
   destruct l2 ; inversion H1 ; subst.
   rewrite 2 app_comm_cons in HP.
-  apply Permutation_cons_app_inv in HP.
+  apply Permutation_Type_cons_app_inv in HP.
   list_simpl in HP.
   apply IHpi in HP.
-  destruct HP as (N & l0 & l1 & Heq' & Htop).
-  exists N.
-  dichot_elt_app_exec Heq' ; subst.
-  + exists l0 ; exists (l4 ++ neg bot :: l3) ; list_simpl ; split...
-  + exists (l2 ++ neg bot :: l5) ; exists l1 ; list_simpl ; split...
+  destruct HP as [(N & l0 & l1) Heq' Htop].
+  dichot_Type_elt_app_exec Heq' ; subst.
+  + exists (N,(l0,l4 ++ neg bot :: l3)) ; list_simpl...
+  + exists (N,(l2 ++ neg bot :: l5,l1)) ; list_simpl...
 - assert (HP' := HP).
   symmetry in HP'.
-  apply Permutation_vs_cons_inv in HP'.
-  destruct HP' as (l2' & l3' & Heq).
+  apply Permutation_Type_vs_cons_inv in HP'.
+  destruct HP' as ((l2' & l3') & Heq).
   destruct l2' ; inversion Heq ; subst.
-  + apply Permutation_cons_inv in HP.
+  + apply Permutation_Type_cons_inv in HP.
     assert (HP' := HP).
-    apply Permutation_vs_cons_inv in HP'.
-    destruct HP' as (l3 & l4 & Heq').
+    apply Permutation_Type_vs_cons_inv in HP'.
+    destruct HP' as ((l3 & l4) & Heq').
     rewrite Heq' in HP.
     symmetry in HP.
-    apply Permutation_cons_app_inv in HP.
-    dichot_app_exec Heq' ;
-      [ | destruct l0 ; inversion Heq'1 ; list_simpl in Heq'1 ] ; subst.
+    apply Permutation_Type_cons_app_inv in HP.
+    dichot_Type_app_exec Heq' ;
+      [ | destruct l0 ; inversion Heq'1 ; list_simpl in Heq'1 ] ;
+        simpl in Heq'0 ; subst.
     * list_simpl in HP.
-      assert (Permutation (pos Q :: l ++ pos Q' :: l4)
-                          (pos Q :: pos Q' :: l ++ l4))
-        as HP' by perm_solve.
+      assert (Permutation_Type (pos Q :: l ++ pos Q' :: l4)
+                               (pos Q :: pos Q' :: l ++ l4))
+        as HP' by perm_Type_solve.
       apply IHpi2 in HP'.
-      destruct HP' as (N & l5 & l6 & Heq' & Htop).
-      exists N.
+      destruct HP' as [(N & l5 & l6) Heq' Htop] ; simpl in Heq'.
       rewrite Heq' in HP.
       rewrite app_assoc in HP.
-      apply Permutation_vs_elt_inv in HP.
-      destruct HP as (l7 & l8 & Heq'').
-      exists l7 ; exists l8 ; split...
-    * destruct (IHpi2 Q Q' l4 (Permutation_refl _))
-        as (N & l5 & l6 & Heq' & Htop) ; subst.
-      exists N.
+      apply Permutation_Type_vs_elt_inv in HP.
+      destruct HP as ((l7 & l8) & Heq'').
+      exists (N,(l7,l8))...
+    * destruct (IHpi2 Q Q' l4 (Permutation_Type_refl _))
+        as [(N & l5 & l6) Heq' Htop] ; subst ; simpl in HP.
       rewrite app_assoc in HP.
-      apply Permutation_vs_elt_inv in HP.
-      destruct HP as (l7 & l8 & Heq'').
-      exists l7 ; exists l8 ; split...
-    * assert (Permutation (pos P :: l3 ++ pos Q' :: l0)
-                          (pos P :: pos Q' :: l3 ++ l0))
-        as HP' by perm_solve.
+      apply Permutation_Type_vs_elt_inv in HP.
+      destruct HP as ((l7 & l8) & Heq'').
+      exists (N,(l7,l8))...
+    * assert (Permutation_Type (pos P :: l3 ++ pos Q' :: l0)
+                               (pos P :: pos Q' :: l3 ++ l0))
+        as HP' by perm_Type_solve.
       apply IHpi1 in HP'.
-      destruct HP' as (N & l5 & l6 & Heq' & Htop).
-      exists N.
+      destruct HP' as [(N & l5 & l6) Heq' Htop] ;
+        simpl in Heq' ; simpl in HP.
       rewrite app_assoc in HP.
       rewrite Heq' in HP.
       list_simpl in HP.
-      apply Permutation_vs_elt_inv in HP.
-      destruct HP as (l7 & l8 & Heq'').
-      exists l7 ; exists l8 ; split...
+      apply Permutation_Type_vs_elt_inv in HP.
+      destruct HP as ((l7 & l8) & Heq'').
+      exists (N,(l7,l8))...
   + destruct l2' ; inversion H1 ; subst.
     * rewrite <- (app_nil_l (pos (tens _ _) :: l3')) in HP.
       rewrite (app_comm_cons _ _ (pos P')) in HP.
-      apply Permutation_cons_app_inv in HP.
+      apply Permutation_Type_cons_app_inv in HP.
       list_simpl in HP.
-      assert (HP' := HP).
-      apply Permutation_vs_cons_inv in HP'.
-      destruct HP' as (l4 & l5 & Heq').
-      dichot_app_exec Heq' ;
-        [ | destruct l0 ; inversion Heq'1 ; list_simpl in Heq'1 ] ; subst.
+      destruct (Permutation_Type_vs_cons_inv _ _ _ HP) as ((l4 & l5) & Heq').
+      dichot_Type_app_exec Heq' ;
+        [ | destruct l0 ; inversion Heq'1 ; list_simpl in Heq'1 ] ;
+          simpl in Heq'1 ; simpl in HP ; subst.
       -- symmetry in HP.
          rewrite app_assoc in HP.
-         apply Permutation_cons_app_inv in HP.
+         apply Permutation_Type_cons_app_inv in HP.
          list_simpl in HP.
-         assert (Permutation (pos Q :: l ++ pos P' :: l5)
-                             (pos Q :: pos P' :: l ++ l5))
-           as HP' by perm_solve.
+         assert (Permutation_Type (pos Q :: l ++ pos P' :: l5)
+                                  (pos Q :: pos P' :: l ++ l5))
+           as HP' by perm_Type_solve.
          apply IHpi2 in HP'.
-         destruct HP' as (N & l6 & l7 & Heq' & Htop).
-         exists N.
+         destruct HP' as [(N & l6 & l7) Heq' Htop].
          rewrite Heq' in HP.
          rewrite app_assoc in HP.
-         apply Permutation_vs_elt_inv in HP.
-         destruct HP as (l8 & l9 & Heq'').
-         exists l8 ; exists l9 ; split...
-      -- destruct (IHpi2 Q P' l5 (Permutation_refl _))
-           as (N & l6 & l7 & Heq' & Htop) ; subst.
-         exists N.
+         apply Permutation_Type_vs_elt_inv in HP.
+         destruct HP as ((l8 & l9) & Heq'').
+         exists (N,(l8,l9))...
+      -- destruct (IHpi2 Q P' l5 (Permutation_Type_refl _))
+           as [(N & l6 & l7) Heq' Htop] ; subst.
          list_simpl in HP.
          symmetry in HP.
-         apply Permutation_cons_app_inv in HP.
+         apply Permutation_Type_cons_app_inv in HP.
          rewrite app_assoc in HP.
-         apply Permutation_vs_elt_inv in HP.
-         destruct HP as (l8 & l9 & Heq'').
-         exists l8 ; exists l9 ; split...
-      -- assert (Permutation (pos P :: l4 ++ pos P' :: l0)
-                             (pos P :: pos P' :: l4 ++ l0))
-           as HP' by perm_solve.
+         apply Permutation_Type_vs_elt_inv in HP.
+         destruct HP as ((l8 & l9) & Heq'').
+         exists (N,(l8,l9))...
+      -- assert (Permutation_Type (pos P :: l4 ++ pos P' :: l0)
+                                  (pos P :: pos P' :: l4 ++ l0))
+           as HP' by perm_Type_solve.
          apply IHpi1 in HP'.
-         destruct HP' as (N & l6 & l7 & Heq' & Htop).
-         exists N.
+         destruct HP' as [(N & l6 & l7) Heq' Htop].
          list_simpl in HP.
          symmetry in HP.
-         apply Permutation_cons_app_inv in HP.
+         apply Permutation_Type_cons_app_inv in HP.
          rewrite app_assoc in HP.
          rewrite Heq' in HP.
          list_simpl in HP.
-         apply Permutation_vs_elt_inv in HP.
-         destruct HP as (l8 & l9 & Heq'').
-         exists l8 ; exists l9 ; split...
+         apply Permutation_Type_vs_elt_inv in HP.
+         destruct HP as ((l8 & l9) & Heq'').
+         exists (N,(l8,l9))...
     * rewrite 2 (app_comm_cons _ (pos (tens _ _) :: l3')) in HP.
-      apply Permutation_cons_app_inv in HP.
+      apply Permutation_Type_cons_app_inv in HP.
       list_simpl in HP.
-      assert (HP' := HP).
-      apply Permutation_vs_cons_inv in HP'.
-      destruct HP' as (l4 & l5 & Heq').
-      dichot_app_exec Heq' ; subst.
-      -- assert (Permutation (pos Q :: l ++ pos P' :: l5)
-                             (pos Q :: pos P' :: l ++ l5))
-           as HP' by perm_solve.
+      destruct (Permutation_Type_vs_cons_inv _ _ _ HP) as ((l4 & l5) & Heq').
+      dichot_Type_app_exec Heq' ; subst.
+      -- assert (Permutation_Type (pos Q :: l ++ pos P' :: l5)
+                                  (pos Q :: pos P' :: l ++ l5))
+           as HP' by perm_Type_solve.
          apply IHpi2 in HP'.
-         destruct HP' as (N & l6 & l7 & Heq' & Htop).
-         exists N.
+         destruct HP' as [(N & l6 & l7) Heq' Htop].
          symmetry in HP.
          rewrite app_assoc in HP.
-         apply Permutation_cons_app_inv in HP.
+         apply Permutation_Type_cons_app_inv in HP.
          list_simpl in HP.
          rewrite Heq' in HP.
          rewrite app_assoc in HP.
-         apply Permutation_vs_elt_inv in HP.
-         destruct HP as (l8 & l9 & Heq'').
+         apply Permutation_Type_vs_elt_inv in HP.
+         destruct HP as ((l8 & l9) & Heq'').
          destruct l8 ; inversion Heq''.
-         dichot_app_exec H2 ;
+         dichot_Type_app_exec H2 ;
            [ | destruct l2 ; inversion Heq'' ; list_simpl in H4 ] ; subst.
-         ++ exists (l2' ++ pos (tens P Q) :: l0) ; exists l9 ;
-              list_simpl ; split...
-         ++ exists (l8 ++ pos (tens P Q) :: nil) ; exists l9 ;
-              list_simpl ; split...
+         ++ exists (N,(l2' ++ pos (tens P Q) :: l0,l9)) ; list_simpl...
+         ++ exists (N,(l8 ++ pos (tens P Q) :: nil,l9)) ; list_simpl...
          ++ inversion H4 ; subst.
-            exists l8 ; exists (l2 ++ pos (tens P Q) :: l3') ;
-              list_simpl ; split...
+            exists (N,(l8,l2 ++ pos (tens P Q) :: l3')) ; list_simpl...
       -- destruct l0 ; inversion Heq'1 ; list_simpl in Heq'1 ; subst.
-         ++ destruct (IHpi2 Q P' l5 (Permutation_refl _))
-              as (N & l6 & l7 & Heq' & Htop) ; subst.
-            exists N.
+         ++ destruct (IHpi2 Q P' l5 (Permutation_Type_refl _))
+              as [(N & l6 & l7) Heq' Htop] ; subst.
             list_simpl in HP.
             symmetry in HP.
-            apply Permutation_cons_app_inv in HP.
+            apply Permutation_Type_cons_app_inv in HP.
             rewrite app_assoc in HP.
-            apply Permutation_vs_elt_inv in HP.
-            destruct HP as (l8 & l9 & Heq'').
+            apply Permutation_Type_vs_elt_inv in HP.
+            destruct HP as ((l8 & l9) & Heq'').
             destruct l8 ; inversion Heq'' ; subst.
-            dichot_app_exec H3 ;
+            dichot_Type_app_exec H3 ;
               [ | destruct l0 ; inversion H2 ; list_simpl in H2 ] ; subst.
-            ** exists (l2' ++ pos (tens P Q) :: l) ; exists l9 ;
-                 list_simpl ; split...
-            ** exists (l8 ++ pos (tens P Q) :: nil) ; exists l9 ;
-                 list_simpl ; split...
-            ** exists l8 ; exists (l0 ++ pos (tens P Q) :: l3') ;
-                 list_simpl ; split...
-         ++ assert (Permutation (pos P :: l4 ++ pos P' :: l0)
-                                (pos P :: pos P' :: l4 ++ l0))
-              as HP' by perm_solve.
+            ** exists (N,(l2' ++ pos (tens P Q) :: l,l9)) ; list_simpl...
+            ** exists (N,(l8 ++ pos (tens P Q) :: nil,l9)) ; list_simpl...
+            ** exists (N,(l8,l0 ++ pos (tens P Q) :: l3')) ; list_simpl...
+         ++ assert (Permutation_Type (pos P :: l4 ++ pos P' :: l0)
+                                     (pos P :: pos P' :: l4 ++ l0))
+              as HP' by perm_Type_solve.
             apply IHpi1 in HP'.
-            destruct HP' as (N & l6 & l7 & Heq' & Htop).
-            exists N.
+            destruct HP' as [(N & l6 & l7) Heq' Htop].
             symmetry in HP.
             list_simpl in HP.
-            apply Permutation_cons_app_inv in HP.
+            apply Permutation_Type_cons_app_inv in HP.
             rewrite app_assoc in HP.
             rewrite Heq' in HP.
             list_simpl in HP.
-            apply Permutation_vs_elt_inv in HP.
-            destruct HP as (l8 & l9 & Heq'').
+            apply Permutation_Type_vs_elt_inv in HP.
+            destruct HP as ((l8 & l9) & Heq'').
             destruct l8 ; inversion Heq''.
-            dichot_app_exec H2 ; 
+            dichot_Type_app_exec H2 ; 
               [ | destruct l1 ; inversion H4 ; list_simpl in H4 ] ; subst.
-            ** exists (l2' ++ pos (tens P Q) :: l) ; exists l9 ;
-                 list_simpl ; split...
-            ** exists (l8 ++ pos (tens P Q) :: nil) ; exists l9 ;
-                 list_simpl ; split...
-            ** exists l8 ; exists (l1 ++ pos (tens P Q) :: l3') ;
-                 list_simpl ; split...
+            ** exists (N,(l2' ++ pos (tens P Q) :: l,l9)) ; list_simpl...
+            ** exists (N,(l8 ++ pos (tens P Q) :: nil,l9)) ; list_simpl...
+            ** exists (N,(l8,l1 ++ pos (tens P Q) :: l3')) ; list_simpl...
 - assert (HP' := HP).
   symmetry in HP'.
-  apply Permutation_vs_cons_inv in HP'.
-  destruct HP' as (l2 & l3 & Heq).
+  apply Permutation_Type_vs_cons_inv in HP'.
+  destruct HP' as ((l2 & l3) & Heq).
   destruct l2 ; inversion Heq.
   destruct l2 ; inversion H1 ; subst.
   rewrite 2 app_comm_cons in HP.
-  apply Permutation_cons_app_inv in HP.
-  apply (Permutation_cons_app _ _ (neg M)) in HP.
-  apply (Permutation_cons_app _ _ (neg N)) in HP.
+  apply Permutation_Type_cons_app_inv in HP.
+  apply (Permutation_Type_cons_app _ _ (neg M)) in HP.
+  apply (Permutation_Type_cons_app _ _ (neg N)) in HP.
   list_simpl in HP.
   apply IHpi in HP.
-  destruct HP as (N' & l0 & l1 & Heq' & Htop).
-  dichot_elt_app_exec Heq' ; subst.
+  destruct HP as [(N' & l0 & l1) Heq' Htop].
+  dichot_Type_elt_app_exec Heq' ; subst.
   + destruct l4 ; inversion Heq'1 ; subst.
-    * exists (parr N N') ; exists l2 ; exists l1 ; list_simpl ; split...
+    * exists (parr N N',(l2,l1)) ; list_simpl...
       apply par_rs...
-    * exists N' ; exists (l2 ++ neg (parr N M) :: l4) ; exists l1 ;
-        list_simpl ; split...
+    * exists (N',(l2 ++ neg (parr N M) :: l4,l1)) ; list_simpl...
   + destruct l5 ; inversion Heq'1 ; subst.
-    * exists (parr N' M) ; exists l0 ; exists l3 ; list_simpl ; split...
+    * exists (parr N' M,(l0,l3)) ; list_simpl...
       apply par_ls...
-    * exists N' ; exists l0 ; exists (l5 ++ neg (parr N M) :: l3) ;
-        list_simpl ; split...
+    * exists (N',(l0,l5 ++ neg (parr N M) :: l3)) ; list_simpl...
 - symmetry in HP.
-  apply Permutation_vs_cons_inv in HP.
-  destruct HP as (l2 & l3 & Heq).
+  apply Permutation_Type_vs_cons_inv in HP.
+  destruct HP as ((l2 & l3) & Heq).
   destruct l2 ; inversion Heq.
   destruct l2 ; inversion H1 ; subst.
-  exists top ; exists l2 ; exists l3 ; split...
+  exists (top,(l2,l3))...
   apply top_s.
 - assert (HP' := HP).
   symmetry in HP'.
-  apply Permutation_vs_cons_inv in HP'.
-  destruct HP' as (l2 & l3 & Heq).
+  apply Permutation_Type_vs_cons_inv in HP'.
+  destruct HP' as ((l2 & l3) & Heq).
   destruct l2 ; inversion Heq ; subst.
-  + apply Permutation_cons_inv in HP.
-    apply (@Permutation_cons _ _ (pos P) eq_refl) in HP.
+  + apply Permutation_Type_cons_inv in HP.
+    apply (@Permutation_Type_cons _ _ (pos P) eq_refl) in HP.
     apply IHpi in HP.
-    destruct HP as (N & l0 & l1 & Heq' & Htop) ; subst.
-    exists N ; exists l0 ; exists l1 ; split...
+    destruct HP as [(N & l0 & l1) Heq' Htop] ; subst.
+    exists (N,(l0,l1))...
   + destruct l2 ; inversion H1 ; subst.
     * rewrite <- (app_nil_l (pos (aplus _ _) :: l3)) in HP.
       rewrite app_comm_cons in HP.
-      apply Permutation_cons_app_inv in HP.
-      apply (@Permutation_cons _ _ (pos P) eq_refl) in HP.
+      apply Permutation_Type_cons_app_inv in HP.
+      apply (@Permutation_Type_cons _ _ (pos P) eq_refl) in HP.
       list_simpl in HP.
       apply IHpi in HP.
-      destruct HP as (N & l0 & l1 & Heq' & Htop) ; subst.
-      exists N ; exists l0 ; exists l1 ; split...
+      destruct HP as [(N & l0 & l1) Heq' Htop] ; subst.
+      exists (N,(l0,l1))...
     * rewrite 2 app_comm_cons in HP.
-      apply Permutation_cons_app_inv in HP.
-      apply (Permutation_cons_app _ _ (pos P)) in HP.
+      apply Permutation_Type_cons_app_inv in HP.
+      apply (Permutation_Type_cons_app _ _ (pos P)) in HP.
       list_simpl in HP.
       apply IHpi in HP.
-      destruct HP as (N' & l0 & l1 & Heq' & Htop).
-      dichot_elt_app_exec Heq' ; subst.
-      -- exists N' ; exists (l2 ++ pos (aplus P Q) :: l4) ; exists l1 ;
-           list_simpl ; split...
+      destruct HP as [(N' & l0 & l1) Heq' Htop].
+      dichot_Type_elt_app_exec Heq' ; subst.
+      -- exists (N',(l2 ++ pos (aplus P Q) :: l4,l1)) ; list_simpl...
       -- destruct l5 ; inversion Heq'1 ; subst.
-         exists N' ; exists l0 ; exists (l5 ++ pos (aplus P Q) :: l3) ;
-           list_simpl ; split...
+         exists (N',(l0,l5 ++ pos (aplus P Q) :: l3)) ; list_simpl...
 - assert (HP' := HP).
   symmetry in HP'.
-  apply Permutation_vs_cons_inv in HP'.
-  destruct HP' as (l2 & l3 & Heq).
+  apply Permutation_Type_vs_cons_inv in HP'.
+  destruct HP' as ((l2 & l3) & Heq).
   destruct l2 ; inversion Heq ; subst.
-  + apply Permutation_cons_inv in HP.
-    apply (@Permutation_cons _ _ (pos P) eq_refl) in HP.
+  + apply Permutation_Type_cons_inv in HP.
+    apply (@Permutation_Type_cons _ _ (pos P) eq_refl) in HP.
     apply IHpi in HP.
-    destruct HP as (N & l0 & l1 & Heq' & Htop) ; subst.
-    exists N ; exists l0 ; exists l1 ; split...
+    destruct HP as [(N & l0 & l1) Heq' Htop] ; subst.
+    exists (N,(l0,l1))...
   + destruct l2 ; inversion H1 ; subst.
     * rewrite <- (app_nil_l (pos (aplus _ _) :: l3)) in HP.
       rewrite app_comm_cons in HP.
-      apply Permutation_cons_app_inv in HP.
-      apply (@Permutation_cons _ _ (pos P) eq_refl) in HP.
+      apply Permutation_Type_cons_app_inv in HP.
+      apply (@Permutation_Type_cons _ _ (pos P) eq_refl) in HP.
       list_simpl in HP.
       apply IHpi in HP.
-      destruct HP as (N & l0 & l1 & Heq' & Htop) ; subst.
-      exists N ; exists l0 ; exists l1 ; split...
+      destruct HP as [(N & l0 & l1) Heq' Htop] ; subst.
+      exists (N,(l0,l1))...
     * rewrite 2 app_comm_cons in HP.
-      apply Permutation_cons_app_inv in HP.
-      apply (Permutation_cons_app _ _ (pos P)) in HP.
+      apply Permutation_Type_cons_app_inv in HP.
+      apply (Permutation_Type_cons_app _ _ (pos P)) in HP.
       list_simpl in HP.
       apply IHpi in HP.
-      destruct HP as (N' & l0 & l1 & Heq' & Htop).
-      dichot_elt_app_exec Heq' ; subst.
-      -- exists N' ; exists (l2 ++ pos (aplus Q P) :: l4) ; exists l1 ;
-           list_simpl ; split...
+      destruct HP as [(N' & l0 & l1) Heq' Htop].
+      dichot_Type_elt_app_exec Heq' ; subst.
+      -- exists (N',(l2 ++ pos (aplus Q P) :: l4,l1)) ; list_simpl...
       -- destruct l5 ; inversion Heq'1 ; subst.
-         exists N' ; exists l0 ; exists (l5 ++ pos (aplus Q P) :: l3) ;
-           list_simpl ; split...
+         exists (N',(l0,l5 ++ pos (aplus Q P) :: l3)) ; list_simpl...
 - assert (HP' := HP).
   symmetry in HP'.
-  apply Permutation_vs_cons_inv in HP'.
-  destruct HP' as (l2 & l3 & Heq).
+  apply Permutation_Type_vs_cons_inv in HP'.
+  destruct HP' as ((l2 & l3) & Heq).
   destruct l2 ; inversion Heq.
   destruct l2 ; inversion H1 ; subst.
   rewrite 2 app_comm_cons in HP.
-  apply Permutation_cons_app_inv in HP.
-  assert (HP1 := (Permutation_cons_app _ _ (neg N) HP)).
-  assert (HP2 := (Permutation_cons_app _ _ (neg M) HP)).
+  apply Permutation_Type_cons_app_inv in HP.
+  assert (HP1 := (Permutation_Type_cons_app _ _ (neg N) HP)).
+  assert (HP2 := (Permutation_Type_cons_app _ _ (neg M) HP)).
   list_simpl in HP1 ; apply IHpi1 in HP1.
   list_simpl in HP2 ; apply IHpi2 in HP2.
-  destruct HP1 as (N' & l0 & l1 & Heq' & Htop).
-  destruct HP2 as (M' & l0' & l1' & Heq'' & Htop').
-  dichot_elt_app_exec Heq' ; subst.
-  + exists N' ; exists (l2 ++ neg (awith N M) :: l4) ; exists l1 ;
-      list_simpl ; split...
+  destruct HP1 as [(N' & l0 & l1) Heq' Htop].
+  destruct HP2 as [(M' & l0' & l1') Heq'' Htop'].
+  dichot_Type_elt_app_exec Heq' ; subst.
+  + exists (N',(l2 ++ neg (awith N M) :: l4,l1)) ; list_simpl...
   + destruct l5 ; inversion Heq'1 ; subst.
     * list_simpl in Heq''.
-      dichot_elt_app_exec Heq'' ; subst.
-      -- exists M' ; exists (l0 ++ neg (awith N' M) :: l2) ; exists l1' ;
-           list_simpl ; split...
+      dichot_Type_elt_app_exec Heq'' ; subst.
+      -- exists (M',(l0 ++ neg (awith N' M) :: l2,l1')) ; list_simpl...
       -- destruct l3 ; inversion Heq''1 ; subst.
-         ++ exists (awith N' M') ; exists l0' ; exists l1' ;
-              list_simpl ; split...
+         ++ exists (awith N' M',(l0',l1')) ;list_simpl...
             apply with_s...
-         ++ exists M' ; exists l0' ; exists (l3 ++ neg (awith N' M) :: l1) ;
-              list_simpl ; split...
-    * exists N' ; exists l0 ; exists (l5 ++ neg (awith N M) :: l3) ;
-        list_simpl ; split...
+         ++ exists (M',(l0',l3 ++ neg (awith N' M) :: l1)) ; list_simpl...
+    * exists (N',(l0,l5 ++ neg (awith N M) :: l3)) ; list_simpl...
 - exfalso.
   assert (HP' := HP).
   symmetry in HP'.
-  apply Permutation_vs_cons_inv in HP'.
-  destruct HP' as (l2 & l3 & Heq).
+  apply Permutation_Type_vs_cons_inv in HP'.
+  destruct HP' as ((l2 & l3) & Heq).
   destruct l2 ; inversion Heq ; subst.
-  + apply Permutation_cons_inv in HP.
-    apply Permutation_vs_cons_inv in HP.
-    destruct HP as (l2 & l3 & Heq').
+  + apply Permutation_Type_cons_inv in HP.
+    apply Permutation_Type_vs_cons_inv in HP.
+    destruct HP as ((l2 & l3) & Heq').
     symmetry in Heq'.
     decomp_map Heq'.
     discriminate Heq'3.
   + destruct l2 ; inversion H1 ; subst.
     * rewrite <- (app_nil_l (pos (oc _) :: l3)) in HP.
       rewrite app_comm_cons in HP.
-      apply Permutation_cons_app_inv in HP.
-      apply Permutation_vs_cons_inv in HP.
-      destruct HP as (l2' & l3' & Heq').
+      apply Permutation_Type_cons_app_inv in HP.
+      apply Permutation_Type_vs_cons_inv in HP.
+      destruct HP as ((l2' & l3') & Heq').
       symmetry in Heq'.
       decomp_map Heq'.
       discriminate Heq'3.
     * rewrite 2 app_comm_cons in HP.
-      apply Permutation_cons_app_inv in HP.
-      apply Permutation_vs_cons_inv in HP.
-      destruct HP as (l2' & l3' & Heq').
+      apply Permutation_Type_cons_app_inv in HP.
+      apply Permutation_Type_vs_cons_inv in HP.
+      destruct HP as ((l2' & l3') & Heq').
       symmetry in Heq'.
       decomp_map Heq'.
       discriminate Heq'3.
 - assert (HP' := HP).
   symmetry in HP'.
-  apply Permutation_vs_cons_inv in HP'.
-  destruct HP' as (l2 & l3 & Heq).
+  apply Permutation_Type_vs_cons_inv in HP'.
+  destruct HP' as ((l2 & l3) & Heq).
   destruct l2 ; inversion Heq.
   destruct l2 ; inversion H1 ; subst.
   rewrite 2 app_comm_cons in HP.
-  apply Permutation_cons_app_inv in HP.
-  apply (Permutation_cons_app _ _ (pos P)) in HP.
+  apply Permutation_Type_cons_app_inv in HP.
+  apply (Permutation_Type_cons_app _ _ (pos P)) in HP.
   list_simpl in HP.
   apply IHpi in HP.
-  destruct HP as (N' & l0 & l1 & Heq' & Htop).
-  dichot_elt_app_exec Heq' ; subst.
-  + exists N' ; exists (l2 ++ neg (wn P) :: l4) ; exists l1 ;
-      list_simpl ; split...
+  destruct HP as [(N' & l0 & l1) Heq' Htop].
+  dichot_Type_elt_app_exec Heq' ; subst.
+  + exists (N',(l2 ++ neg (wn P) :: l4,l1)) ; list_simpl...
   + destruct l5 ; inversion Heq'1 ; subst.
-    exists N' ; exists l0 ; exists (l5 ++ neg (wn P) :: l3) ;
-      list_simpl ; split...
+    exists (N',(l0,l5 ++ neg (wn P) :: l3)) ; list_simpl...
 - assert (HP' := HP).
   symmetry in HP'.
-  apply Permutation_vs_cons_inv in HP'.
-  destruct HP' as (l2 & l3 & Heq).
+  apply Permutation_Type_vs_cons_inv in HP'.
+  destruct HP' as ((l2 & l3) & Heq).
   destruct l2 ; inversion Heq.
   destruct l2 ; inversion H1 ; subst.
   rewrite 2 app_comm_cons in HP.
-  apply Permutation_cons_app_inv in HP.
+  apply Permutation_Type_cons_app_inv in HP.
   list_simpl in HP.
   apply IHpi in HP.
-  destruct HP as (N & l0 & l1 & Heq' & Htop).
-  exists N.
-  dichot_elt_app_exec Heq' ; subst.
-  + exists l0 ; exists (l4 ++ neg (wn P) :: l3) ; list_simpl ; split...
-  + exists (l2 ++ neg (wn P) :: l5) ; exists l1 ; list_simpl ; split...
+  destruct HP as [(N & l0 & l1) Heq' Htop].
+  dichot_Type_elt_app_exec Heq' ; subst.
+  + exists (N,(l0,l4 ++ neg (wn P) :: l3)) ; list_simpl...
+  + exists (N,(l2 ++ neg (wn P) :: l5,l1)) ; list_simpl...
 - assert (HP' := HP).
   symmetry in HP'.
-  apply Permutation_vs_cons_inv in HP'.
-  destruct HP' as (l2 & l3 & Heq).
+  apply Permutation_Type_vs_cons_inv in HP'.
+  destruct HP' as ((l2 & l3) & Heq).
   destruct l2 ; inversion Heq.
   destruct l2 ; inversion H1 ; subst.
   rewrite 2 app_comm_cons in HP.
-  apply Permutation_cons_app_inv in HP.
-  apply (Permutation_cons_app _ _ (neg (wn P))) in HP.
-  apply (Permutation_cons_app _ _ (neg (wn P))) in HP.
+  apply Permutation_Type_cons_app_inv in HP.
+  apply (Permutation_Type_cons_app _ _ (neg (wn P))) in HP.
+  apply (Permutation_Type_cons_app _ _ (neg (wn P))) in HP.
   list_simpl in HP.
   apply IHpi in HP.
-  destruct HP as (N' & l0 & l1 & Heq' & Htop).
-  dichot_elt_app_exec Heq' ; subst.
+  destruct HP as [(N' & l0 & l1) Heq' Htop].
+  dichot_Type_elt_app_exec Heq' ; subst.
   + destruct l4 ; inversion Heq'1 ; subst.
     * inversion Htop.
-    * exists N' ; exists (l2 ++ neg (wn P) :: l4) ; exists l1 ;
-        list_simpl ; split...
+    * exists (N',(l2 ++ neg (wn P) :: l4,l1)) ; list_simpl...
   + destruct l5 ; inversion Heq'1 ; subst.
     * inversion Htop.
-    * exists N' ; exists l0 ; exists (l5 ++ neg (wn P) :: l3) ;
-        list_simpl ; split...
+    * exists (N',(l0,l5 ++ neg (wn P) :: l3)) ; list_simpl...
 Qed.
 
 Theorem llpol_is_ll_polsequent : forall l,
-  llpol l -> polsequent l -> llpol_ps polsequent l.
+  llpol l -> polsequent l -> llpol_ps polsequent_bool l.
 Proof with try eassumption ; try reflexivity.
 intros l pi.
 induction pi ; intros Hpol.
 - constructor.
+  apply polsequent_true.
   right.
-  exists (covar X :: nil) ; exists (var X).
-  apply perm_swap.
-- eapply ex_ps_r...
+  exists (covar X :: nil,var X).
+  apply Permutation_Type_swap.
+- eapply ex_ps_r ; [ apply polsequent_true | | ]...
   apply IHpi.
-  destruct Hpol as [ (l0 & Heq) | (l0 & P & HP) ] ; subst.
-  + apply Permutation_map_inv in H.
-    destruct H as (l & Heq & _) ; subst.
+  destruct Hpol as [ (l0 & Heq) | ((l0 & P) & HP) ] ; subst.
+  + apply Permutation_Type_map_inv in p.
+    destruct p as [l Heq _] ; subst.
     left ; eexists...
   + assert (HP' := HP).
-    apply Permutation_vs_cons_inv in HP'.
-    destruct HP' as (l3 & l4 & Heq) ; subst.
+    apply Permutation_Type_vs_cons_inv in HP'.
+    destruct HP' as ((l3 & l4) & Heq) ; subst.
     symmetry in HP.
-    apply Permutation_cons_app_inv in HP.
+    apply Permutation_Type_cons_app_inv in HP.
     symmetry in HP.
-    apply Permutation_map_inv in HP.
-    destruct HP as (l & Heq & HP).
-    decomp_map Heq ; subst.
-    right ; exists (l5 ++ l6) ; exists P ; perm_solve.
+    apply Permutation_Type_map_inv in HP.
+    destruct HP as [l Heq HP].
+    decomp_map_Type Heq ; simpl in Heq1 ; simpl in Heq2 ;
+      subst ; simpl in p.
+    right ; exists (l5 ++ l6,P) ; simpl ; perm_Type_solve.
 - constructor.
-  right ; exists nil ; exists one...
-- constructor...
+  apply polsequent_true.
+  right ; exists (nil,one)...
+- constructor ; [ apply polsequent_true | ]...
   apply IHpi.
   eapply polsequent_neg_rem...
 - apply polsequent_pos_rem in Hpol.
   destruct Hpol as [ l' Heq ].
-  decomp_map Heq ; subst.
+  decomp_map_Type Heq ; subst.
   constructor...
-  + right ; exists (l0 ++ l3) ; exists (tens P Q) ; perm_solve.
+  + apply polsequent_true.
+    right ; exists (l0 ++ l3,tens P Q) ; perm_Type_solve.
   + apply IHpi1.
-    right ; exists l0 ; exists P ; perm_solve.
+    right ; exists (l0,P) ; perm_Type_solve.
   + apply IHpi2.
-    right ; exists l3 ; exists Q ; perm_solve.
-- constructor...
+    right ; exists (l3,Q) ; perm_Type_solve.
+- constructor ; [ apply polsequent_true | ]...
   apply IHpi.
   apply polsequent_neg_add.
   apply polsequent_neg_add.
   eapply polsequent_neg_rem...
-- constructor...
+- constructor ; apply polsequent_true...
 - assert (Hpol' := Hpol).
   apply polsequent_pos_rem in Hpol'.
   destruct Hpol' as [ l' Heq ] ; subst.
-  constructor...
+  constructor ; [ apply polsequent_true | ]...
   apply IHpi.
-  right ; exists l' ; exists P ; perm_solve.
+  right ; exists (l',P) ; perm_Type_solve.
 - assert (Hpol' := Hpol).
   apply polsequent_pos_rem in Hpol'.
   destruct Hpol' as [ l' Heq ] ; subst.
-  apply plus_ps_r2...
+  apply plus_ps_r2 ; [ apply polsequent_true | ]...
   apply IHpi.
-  right ; exists l' ; exists P ; perm_solve.
-- constructor...
+  right ; exists (l',P) ; perm_Type_solve.
+- constructor ; [ apply polsequent_true | | ]...
   + apply IHpi1.
     apply polsequent_neg_add.
     eapply polsequent_neg_rem...
   + apply IHpi2.
     apply polsequent_neg_add.
     eapply polsequent_neg_rem...
-- constructor...
+- constructor ; [ apply polsequent_true | ]...
   apply IHpi.
   left ; exists (N :: map wn l)...
-- destruct Hpol as [ (l0 & Heq) | (l0 & Q & HP) ] ; subst.
+- destruct Hpol as [ (l0 & Heq) | ((l0 & Q) & HP) ] ; subst.
   + apply de_ps_r.
-    * left ; rewrite Heq ; eexists...
+    * apply polsequent_true.
+      left ; rewrite Heq ; eexists...
     * apply IHpi...
       destruct l0 ; inversion Heq ; subst.
-      right ; exists l0 ; exists P...
-  + assert (HP' := HP).
-    apply Permutation_vs_cons_inv in HP'.
-    destruct HP' as (l2 & l3 & Heq).
+      right ; exists (l0,P)...
+  + destruct (Permutation_Type_vs_cons_inv _ _ _ HP) as ((l2 & l3) & Heq).
     destruct l2 ; inversion Heq ; subst.
     assert (pi' := pi).
-    apply bipos_top_surf with _ P Q (l2 ++ l3) in pi' ; [ | perm_solve ].
-    destruct pi' as (N & l & l' & Heq' & Htop).
-    apply (ex_r _ (pos P :: pos Q :: l2 ++ l3)) in pi ; [ | perm_solve ].
+    apply bipos_top_surf with _ P Q (l2 ++ l3) in pi' ; [ | perm_Type_solve ].
+    destruct pi' as [(N & l & l') Heq' Htop].
+    apply (ex_r _ (pos P :: pos Q :: l2 ++ l3)) in pi ; [ | perm_Type_solve ].
     rewrite Heq' in pi.
-    apply (ex_r _ (neg N :: pos P :: pos Q :: l ++ l')) in pi ; [ | perm_solve ].
+    apply (ex_r _ (neg N :: pos P :: pos Q :: l ++ l')) in pi ; [ | perm_Type_solve ].
     eapply top_imp_top_surf_ps in Htop.
     * apply (ex_ps_r _ (neg N :: neg (wn P) :: pos Q :: l ++ l'))...
-      -- right ; eexists ; eexists...
+      -- apply polsequent_true.
+         right ; eexists...
       -- transitivity (neg (wn P) :: pos Q :: l2 ++ l3) ;
-           [ rewrite Heq' | ] ; perm_solve.
+           [ rewrite Heq' | ] ; perm_Type_solve.
     * apply (polsequent_neg_rem N).
-      right ; exists l0 ; exists Q.
+      right ; exists (l0,Q).
       etransitivity ; [ | apply HP ].
       transitivity (neg (wn P) :: pos Q :: l2 ++ l3) ;
-        [ rewrite Heq' | ] ; perm_solve.
-- apply wk_ps_r...
+        [ rewrite Heq' | ] ; perm_Type_solve.
+- apply wk_ps_r ; [ apply polsequent_true | ]...
   apply IHpi.
   eapply polsequent_neg_rem...
-- apply co_ps_r...
+- apply co_ps_r ; [ apply polsequent_true | ]...
   apply IHpi.
   apply polsequent_neg_add...
 Qed.
 
 (** [llpol] with [top] rule constrained to at most one positive formula. *)
-Inductive llpolt : list formula -> Prop :=
+Inductive llpolt : list formula -> Type :=
 | ax_rt : forall X, llpolt (neg (covar X) :: pos (var X) :: nil)
 | ex_rt : forall l1 l2, llpolt l1 ->
-               Permutation l1 l2 -> llpolt l2
+               Permutation_Type l1 l2 -> llpolt l2
 | one_rt : llpolt (pos one :: nil)
 | bot_rt : forall l, llpolt l -> llpolt (neg bot :: l)
 | tens_rt : forall P Q l1 l2,
@@ -1188,67 +1374,72 @@ Inductive llpolt : list formula -> Prop :=
                llpolt (neg (wn P) :: neg (wn P) :: l) ->
                llpolt (neg (wn P) :: l).
 
-Instance llpolt_perm : Proper ((@Permutation _) ==> Basics.impl) llpolt.
+Instance llpolt_perm : Proper ((@Permutation_Type _) ==> Basics.arrow) llpolt.
 Proof.
 intros l1 l2 HP pi.
 eapply ex_rt ; eassumption.
 Qed.
 
 (** For polarized sequents [llpol] corresponds to [top] rule with at most one positive formula. *)
-Theorem llpol_llpolt : forall l, (polsequent l /\ llpol l) <-> llpolt l.
+Theorem llpol_llpolt : forall l, polsequent l -> llpol l -> llpolt l.
 Proof with try eassumption ; try reflexivity.
-intros l ; split.
-- intros [ Hpol pi ].
-  apply llpol_is_ll_polsequent in pi...
-  clear Hpol ; induction pi ; try (now constructor).
-  + eapply ex_rt...
-  + apply top_rt.
-    eapply polsequent_neg_rem...
-- intros pi.
-  induction pi ; (split ; [ | try (now constructor) ]) ;
-    try (destruct IHpi as [Hpol pi']) ;
-    try (destruct IHpi1 as [Hpol1 pi1']) ;
-    try (destruct IHpi2 as [Hpol2 pi2'])...
-  + right ; exists (covar X :: nil) ; exists (var X) ; perm_solve.
-  + destruct Hpol.
-    * destruct H0 as [l0 H0] ; subst.
-      symmetry in H.
-      apply Permutation_map_inv in H.
-      destruct H as (l3 & Heq & HP) ; subst.
-      left ; exists l3...
-    * destruct H0 as (l0 & P & H0) ; subst.
-      assert (HP := H0).
-      apply Permutation_vs_cons_inv in H0.
-      destruct H0 as (l3 & l4 & Heq) ; subst.
-      symmetry in HP.
-      apply Permutation_cons_app_inv in HP.
-      right ; exists l0 ; exists P ; perm_solve.
-  + eapply ex_r...
-  + right ; exists nil ; exists one ; perm_solve.
-  + apply polsequent_neg_add...
-  + apply polsequent_pos_rem in Hpol1.
-    destruct Hpol1 as [l1' Heq] ; subst.
-    apply polsequent_pos_rem in Hpol2.
-    destruct Hpol2 as [l2' Heq] ; subst.
-    right ; exists (l1' ++ l2') ; exists (tens P Q) ; perm_solve.
-  + apply polsequent_neg_rem in Hpol.
-    apply polsequent_neg_rem in Hpol.
-    eapply polsequent_neg_add...
-  + eapply polsequent_neg_add...
-  + apply polsequent_pos_rem in Hpol.
-    destruct Hpol as [l' Heq] ; subst.
-    right ; exists l' ; exists (aplus P Q) ; perm_solve.
-  + apply polsequent_pos_rem in Hpol.
-    destruct Hpol as [l' Heq] ; subst.
-    right ; exists l' ; exists (aplus Q P) ; perm_solve.
-  + apply polsequent_neg_rem in Hpol1.
-    eapply polsequent_neg_add...
-  + right ; exists (map wn l) ; exists (oc N) ; perm_solve.
-  + apply polsequent_pos_rem in Hpol.
-    destruct Hpol as [l' Heq] ; subst.
-    left ; exists (wn P :: l')...
-  + eapply polsequent_neg_add...
-  + eapply polsequent_neg_rem...
+intros l Hpol pi.
+apply llpol_is_ll_polsequent in pi...
+clear Hpol ; induction pi ; try (now constructor).
+- eapply ex_rt...
+- apply true_polsequent in i.
+  apply top_rt.
+  eapply polsequent_neg_rem...
+Qed.
+
+Theorem llpolt_llpol : forall l, llpolt l -> (polsequent l * llpol l).
+Proof with try eassumption ; try reflexivity.
+intros l pi.
+induction pi ; split ;
+  try (destruct IHpi as [Hpol pi']) ;
+  try (destruct IHpi1 as [Hpol1 pi1']) ;
+  try (destruct IHpi2 as [Hpol2 pi2']) ;
+  try now constructor...
+- right ; exists (covar X :: nil,var X) ; perm_Type_solve.
+- destruct Hpol.
+  + destruct s as [l0 H0] ; subst.
+    symmetry in p.
+    apply Permutation_Type_map_inv in p.
+    destruct p as [l3 Heq HP] ; subst.
+    left ; exists l3...
+  + destruct s as ((l0 & P) & H0) ; subst.
+    assert (HP := H0).
+    apply Permutation_Type_vs_cons_inv in H0.
+    destruct H0 as ((l3 & l4) & Heq) ; subst.
+    symmetry in HP.
+    apply Permutation_Type_cons_app_inv in HP.
+    right ; exists (l0,P) ; perm_Type_solve.
+- eapply ex_r...
+- right ; exists (nil,one) ; perm_Type_solve.
+- apply polsequent_neg_add...
+- apply polsequent_pos_rem in Hpol1.
+  destruct Hpol1 as [l1' Heq] ; subst.
+  apply polsequent_pos_rem in Hpol2.
+  destruct Hpol2 as [l2' Heq] ; subst.
+  right ; exists (l1' ++ l2',tens P Q) ; perm_Type_solve.
+- apply polsequent_neg_rem in Hpol.
+  apply polsequent_neg_rem in Hpol.
+  eapply polsequent_neg_add...
+- eapply polsequent_neg_add...
+- apply polsequent_pos_rem in Hpol.
+  destruct Hpol as [l' Heq] ; subst.
+  right ; exists (l',aplus P Q) ; perm_Type_solve.
+- apply polsequent_pos_rem in Hpol.
+  destruct Hpol as [l' Heq] ; subst.
+  right ; exists (l',aplus Q P) ; perm_Type_solve.
+- apply polsequent_neg_rem in Hpol1.
+  eapply polsequent_neg_add...
+- right ; exists (map wn l,oc N) ; perm_Type_solve.
+- apply polsequent_pos_rem in Hpol.
+  destruct Hpol as [l' Heq] ; subst.
+  left ; exists (wn P :: l')...
+- eapply polsequent_neg_add...
+- eapply polsequent_neg_rem...
 Qed.
 
 
